@prefix rdf: <http://www.w3.org/1999/02/22-rdf-syntax-ns#> .
@prefix rdfs: <http://www.w3.org/2000/01/rdf-schema#> .
@prefix owl: <http://www.w3.org/2002/07/owl#> .
@prefix xml: <http://www.w3.org/XML/1998/namespace> .
@prefix xsd: <http://www.w3.org/2001/XMLSchema#> .
@prefix dul: <http://www.loa-cnr.it/ontologies/DUL.owl#> .
@prefix skos: <http://www.w3.org/2004/02/skos/core#> .
@prefix vann: <http://purl.org/vocab/vann/> .
@prefix void: <http://rdfs.org/ns/void#> .
@prefix vcard: <http://www.w3.org/2006/vcard/ns#> .
@prefix dcterms: <http://purl.org/dc/terms/> .
@prefix dce: <http://purl.org/dc/elements/1.1/> .
@prefix foaf: <http://xmlns.com/foaf/spec/> .
@prefix om: <http://www.wurvoc.org/vocabularies/om-1.8/> .
@prefix geo: <http://www.w3.org/2003/01/geo/wgs84_pos#> .
@prefix prov: <http://www.w3.org/ns/prov#> .
@prefix obda: <https://w3id.org/obda/vocabulary#> .
@prefix ssn: <http://purl.oclc.org/NET/ssnx/ssn#> .
@prefix sto: <https://w3id.org/i40/sto#> .
@prefix aas: <https://admin-shell.io/aas/2/0/rdf#> .
@base <https://admin-shell.io/aas/2/0/rdf> .

aas: rdf:type owl:Ontology ;
        rdfs:comment "Update implementing the specifiations coming from 'Details of the Asset Administration Shell - Part 1: The exchange of information between partners in the value chain of Industrie 4.0 (Version 2.0)'" ;
        vann:preferredNamespaceUri "https://www.admin-shell.io/aas/2/0/rdf#" ;
        owl:versionInfo 2.0 ;
        skos:definition "An Ontology to represents the Reference Architecture Model for Industry 4.0 (RAMI), including the concept of the Administration Shell I4.0 Component."@en ;
        void:vocabulary rdfs: ,
                      skos: ,
                      dce: ;
        skos:prefLabel "aas"@en ;
        void:vocabulary xsd: ;
        vann:preferredNamespacePrefix "aas" ;
        rdfs:isDefinedBy <https://admin-shell.io/aas/2/0/rdf#> ;
        dcterms:creator <https://www.linkedin.com/in/irl%C3%A1n-g-51766139/> ;
        dcterms:creator <https://www.linkedin.com/in/sebastianrbader/> ;
.
                              

#################################################################
#    Annotation properties
#################################################################

###  http://purl.org/dc/elements/1.1/date
dce:date rdf:type owl:AnnotationProperty .


###  http://purl.org/dc/elements/1.1/description
dce:description rdf:type owl:AnnotationProperty .


###  http://purl.org/dc/elements/1.1/format
dce:format rdf:type owl:AnnotationProperty .


###  http://purl.org/dc/elements/1.1/identifier
dce:identifier rdf:type owl:AnnotationProperty .


###  http://purl.org/dc/elements/1.1/language
dce:language rdf:type owl:AnnotationProperty .


###  http://purl.org/dc/elements/1.1/relation
dce:relation rdf:type owl:AnnotationProperty .


###  http://purl.org/dc/elements/1.1/source
dce:source rdf:type owl:AnnotationProperty .


###  http://purl.org/dc/terms/description
dcterms:description rdf:type owl:AnnotationProperty .


###  http://purl.org/dc/terms/identifier
dcterms:identifier rdf:type owl:AnnotationProperty ;
                   rdfs:subPropertyOf dce:identifier ;
                   rdfs:range rdfs:Literal .


###  http://purl.org/vocab/vann/preferredNamespacePrefix
vann:preferredNamespacePrefix rdf:type owl:AnnotationProperty .


###  http://purl.org/vocab/vann/preferredNamespaceUri
vann:preferredNamespaceUri rdf:type owl:AnnotationProperty .


###  http://rdfs.org/ns/void#vocabulary
void:vocabulary rdf:type owl:AnnotationProperty .


###  http://www.w3.org/2004/02/skos/core#altLabel
skos:altLabel rdf:type owl:AnnotationProperty .


###  http://www.w3.org/2004/02/skos/core#definition
skos:definition rdf:type owl:AnnotationProperty .


###  http://www.w3.org/2004/02/skos/core#note
skos:note rdf:type owl:AnnotationProperty .


###  http://www.w3.org/2004/02/skos/core#prefLabel
skos:prefLabel rdf:type owl:AnnotationProperty .


###  http://www.wurvoc.org/vocabularies/om-1.8/hasNumericalValue
om:hasNumericalValue rdf:type owl:DatatypeProperty ;
                     rdfs:domain om:Measure .


###  https://admin-shell.io/aas/2/0/rdf#assetId
aas:assetId rdf:type owl:DatatypeProperty ;
             rdfs:domain aas:Asset .


###  https://admin-shell.io/aas/2/0/rdf#description
aas:description rdf:type owl:AnnotationProperty ;
                 rdfs:subPropertyOf rdfs:comment ;
                 rdfs:range xsd:string ;
                 rdfs:domain aas:Asset .


###  https://admin-shell.io/aas/2/0/rdf#display
aas:display rdf:type owl:AnnotationProperty .


###  https://admin-shell.io/aas/2/0/rdf#idShort
aas:idShort rdf:type owl:AnnotationProperty .


###  https://admin-shell.io/aas/2/0/rdf#semanticId
aas:semanticId rdf:type owl:AnnotationProperty ;
                rdfs:subPropertyOf rdfs:seeAlso ;
                rdfs:range aas:ExpressionSemantic ;
                rdfs:domain aas:Submodel .


#################################################################
#    Datatypes
#################################################################

###  http://www.w3.org/2001/XMLSchema#date
xsd:date rdf:type rdfs:Datatype .


###  https://admin-shell.io/aas/2/0/rdf#IRDI
aas:IRDI rdf:type rdfs:Datatype ;
          rdfs:comment """IRDI - ISO29002-5, ISO IEC 6523 and ISO IEC 11179-6 [20] as an Identifier scheme for properties and classifications. They are created in a process of consortium-wise specification or international standardisation.
To this end, users sit down together and feed their ideas into the consortia or standardisation bodies. Properties in ISO, IEC help to safeguard key commercial interests. Repositories like eCl@ss and others make it possible to standardise a relatively large number of Identifiers in an appropriately short time."""@en .


###  https://admin-shell.io/aas/2/0/rdf#blob
aas:blob rdf:type rdfs:Datatype ;
          rdfs:comment "A BLOB is a data element that represents a file that is contained with its source code in the value attribute."@en ;
          rdfs:label "aas:blob"^^xsd:string .


###  https://admin-shell.io/aas/2/0/rdf#file
aas:file rdf:type rdfs:Datatype ;
          rdfs:comment "A File is a data element that represents a file via its path description."@en ;
          rdfs:label "aas:file"^^xsd:string .


#################################################################
#    Object Properties
#################################################################

###  http://www.loa-cnr.it/ontologies/DUL.owl#isPartOf
dul:isPartOf rdf:type owl:ObjectProperty ,
                      owl:TransitiveProperty ;
             rdfs:domain aas:Asset ;
             rdfs:range aas:Asset ;
             rdfs:comment "A relation between any entities, in this case, the Asset can be part of other Asset(s)."^^xsd:string ;
             rdfs:isDefinedBy <http://www.ontologydesignpatterns.org/ont/dul/DUL.owl> ;
             rdfs:label "is Part Of"@en .


###  http://www.w3.org/TR/2013/REC-prov-o-20130430/#wasDerivedFrom
<http://www.w3.org/TR/2013/REC-prov-o-20130430/#wasDerivedFrom> rdf:type owl:ObjectProperty ;
                                                                rdfs:subPropertyOf owl:topObjectProperty .


###  https://admin-shell.io/aas/2/0/rdf#administration
aas:administration rdf:type owl:ObjectProperty ;
                    rdfs:comment """Administrative information of an identifiable element.
Note: Some of the administrative information like the version number might
need to be part of the identification."""@en ;
                    rdfs:label "has administration"@en .


###  https://admin-shell.io/aas/2/0/rdf#asset
aas:asset rdf:type owl:ObjectProperty ;
           rdfs:domain aas:AdminShell ;
           rdfs:range aas:Asset ;
           rdfs:comment "The asset the AAS is representing."@en ;
           rdfs:label "asset"@en .


###  https://admin-shell.io/aas/2/0/rdf#assetIdentificationModel
aas:assetIdentificationModel rdf:type owl:ObjectProperty ;
                              rdfs:subPropertyOf aas:hasSubmodel ;
                              rdfs:domain aas:Asset ;
                              rdfs:range aas:Submodel ;
                              rdfs:comment """A reference to a Submodel that defines the handling of
additional domain specific (proprietary) Identifiers for
the asset like e.g. serial number etc."""@en ;
                              rdfs:label "has Asset Identification Model"^^xsd:string .


###  https://admin-shell.io/aas/2/0/rdf#conceptDictionary
aas:conceptDictionary rdf:type owl:ObjectProperty ;
                       rdfs:domain aas:AdminShell ;
                       rdfs:range aas:ConceptDictionary ;
                       rdfs:comment "An AAS max have one or more concept dictionaries assigned to it. The concept dictionaries typically contain only descriptions for elements that are also used within the AAS (via HasSemantics)."@en ;
                       rdfs:label "has concept dictionary" .


###  https://admin-shell.io/aas/2/0/rdf#containedElement
aas:containedElement rdf:type owl:ObjectProperty ;
                      rdfs:comment "Referable elements that are contained in the view."@en ;
                      rdfs:label "containedElement"^^xsd:string .


###  https://admin-shell.io/aas/2/0/rdf#contributes
aas:contributes rdf:type owl:ObjectProperty ;
                 rdfs:domain aas:Submodel ;
                 skos:definition "Agent(Person or Software) that contributes to the Entity/Object related data. It correspond to the Contributor concept of OMM"@en ;
                 skos:prefLabel "has Type Description"@en .


###  https://admin-shell.io/aas/2/0/rdf#dataElement
aas:dataElement rdf:type owl:ObjectProperty ;
                 rdfs:comment """A data element is a submodel element that is not further composed out of other submodel elements.
A data element is a submodel element that has a value. The type of value differs for different subtypes of data elements."""@en ;
                 rdfs:label "dataElement"@en .


###  https://admin-shell.io/aas/2/0/rdf#defaultEnvironmentAttributes
aas:defaultEnvironmentAttributes rdf:type owl:ObjectProperty ;
                                  rdfs:comment """Reference to a submodel defining default environment attributes, i.e. attributes that are not describing the asset itself.
The submodel is of kind=Type.
At the same type the values of these environment attributes need to be accessible when evaluating the access permission rules. This is realized as a policy information point."""@en ;
                                  rdfs:label "defaultEnvironmentAttributes"^^xsd:string .


###  https://admin-shell.io/aas/2/0/rdf#defaultPermissions
aas:defaultPermissions rdf:type owl:ObjectProperty ;
                        rdfs:comment "Reference to a submodel defining the default permissions for the AAS."@en ;
                        rdfs:label "defaultPermissions"^^xsd:string .


###  https://admin-shell.io/aas/2/0/rdf#defaultSubjectAttributes
aas:defaultSubjectAttributes rdf:type owl:ObjectProperty ;
                              rdfs:comment """Reference to a submodel defining the default subjects attributes for the AAS that can be used to describe access permission rules.
The submodel is of kind=Type."""@en ;
                              rdfs:label "defaultSubjectAttributes"^^xsd:string .


###  https://admin-shell.io/aas/2/0/rdf#dependsOn
aas:dependsOn rdf:type owl:ObjectProperty ;
               rdfs:comment "A formula may depend on referable or even external global elements - assumed that can be referenced and their value may be evaluated - that are used in the logical expression."@en ;
               rdfs:label "dependsOn"@en .


###  https://admin-shell.io/aas/2/0/rdf#derivedFrom
aas:derivedFrom rdf:type owl:ObjectProperty ;
                 rdfs:subPropertyOf <http://www.w3.org/TR/2013/REC-prov-o-20130430/#wasDerivedFrom> ;
                 rdfs:domain aas:AdminShell ;
                 rdfs:range aas:AdminShell ;
                 rdfs:comment "This relation connects instances of AAS with their respective types. Refer to Asset Kind for further information of instance and type kinds."@en ;
                 rdfs:label "derived from"^^xsd:string .


###  https://admin-shell.io/aas/2/0/rdf#describes
aas:describes rdf:type owl:ObjectProperty ;
               rdfs:domain aas:AdminShell ;
               rdfs:range aas:Asset ;
               rdfs:comment "Connect the Asset with the Administration Shell"@en ;
               skos:altLabel "describes"@en .


###  https://admin-shell.io/aas/2/0/rdf#first
aas:first rdf:type owl:ObjectProperty ;
           rdfs:comment "First element in the relationship taking the role of the subject."@en ;
           rdfs:label "first"^^xsd:string .


###  https://admin-shell.io/aas/2/0/rdf#hasConceptDescription
aas:hasConceptDescription rdf:type owl:ObjectProperty ;
                           rdfs:comment """The semantics of a property or other elements that may have a semantic description is defined by a concept description.
The description of the concept should follow a standardized schema (realized as data specification template)."""@en ;
                           rdfs:label "has ConceptDescription"@en .


###  https://admin-shell.io/aas/2/0/rdf#hasDataSpecification
aas:hasDataSpecification rdf:type owl:ObjectProperty ;
                          rdfs:subPropertyOf owl:topObjectProperty ;
                          rdfs:comment "Global reference to the data specification template used by the element."@en ;
                          rdfs:label "has Data Specification"@en .


###  https://admin-shell.io/aas/2/0/rdf#hasDatatype
aas:hasDatatype rdf:type owl:ObjectProperty ;
                 rdfs:domain aas:Submodel ;
                 rdfs:comment "Points to the datatypes of the Submodels"@en ;
                 rdfs:label "has Datatype"@en .


###  https://admin-shell.io/aas/2/0/rdf#hasIdType
aas:hasIdType rdf:type owl:ObjectProperty ;
               rdfs:comment """Type of the key value.
In case of idType = idShort local shall be true.
In case type=GlobalReference idType shall not be IdShort."""@en ;
               rdfs:label "has idType"@en .


###  https://admin-shell.io/aas/2/0/rdf#hasKey
aas:hasKey rdf:type owl:ObjectProperty ;
            rdfs:comment "Unique reference in its name space."@en ;
            rdfs:label "has Key"^^xsd:string .


###  https://admin-shell.io/aas/2/0/rdf#hasKind
aas:hasKind rdf:type owl:ObjectProperty ;
             rdfs:subPropertyOf owl:topObjectProperty ;
             rdfs:domain aas:AdminShell ;
             rdfs:range aas:AssetKind ;
             rdfs:label "has kind"@en .


###  https://admin-shell.io/aas/2/0/rdf#hasReference
aas:hasReference rdf:type owl:ObjectProperty ;
                  rdfs:domain aas:Submodel ;
                  rdfs:label "has Reference"@en .


###  https://admin-shell.io/aas/2/0/rdf#hasSubjectAttribute
aas:hasSubjectAttribute rdf:type owl:ObjectProperty ;
                         rdfs:comment "A data element that further classifies a specific subject."@en ;
                         rdfs:label "has subjectAttribute"^^xsd:string .


###  https://admin-shell.io/aas/2/0/rdf#hasSubmodel
aas:hasSubmodel rdf:type owl:ObjectProperty ;
                 rdfs:domain aas:Asset ;
                 rdfs:range aas:Submodel ;
                 rdfs:comment "Points to the Admin Shell to the Submodels that describe the Admin Shell of a given Asset"@en ;
                 rdfs:label "has Submodel"@en ;
                 skos:altLabel "assetIdentificationModel"@en .


###  https://admin-shell.io/aas/2/0/rdf#hasValue
aas:hasValue rdf:type owl:ObjectProperty ;
              rdfs:domain aas:Submodel ;
              rdfs:range aas:Value .


###  https://admin-shell.io/aas/2/0/rdf#hasView
aas:hasView rdf:type owl:ObjectProperty ;
             rdfs:domain aas:AdminShell ;
             rdfs:range aas:View ;
             rdfs:comment "Points to the differents views associated to the Administration Shell via the Submodels."@en ;
             rdfs:label "has View"@en ;
             skos:prefLabel "view"@en .


###  https://admin-shell.io/aas/2/0/rdf#in
aas:in rdf:type owl:ObjectProperty ;
        rdfs:comment "the aas:in attribute of aas:operation is the input parameter"@en .


###  https://admin-shell.io/aas/2/0/rdf#inAccordanceWith
aas:inAccordanceWith rdf:type owl:ObjectProperty ;
                      rdfs:domain aas:Submodel ;
                      rdfs:comment "The Submodel is in accordance with a given standard specified in the STO ontology"@en ;
                      rdfs:label "in Accordance With"@en .


###  https://admin-shell.io/aas/2/0/rdf#isCaseOf
aas:isCaseOf rdf:type owl:ObjectProperty .


###  https://admin-shell.io/aas/2/0/rdf#isConnectedTo
aas:isConnectedTo rdf:type owl:ObjectProperty ;
                   rdfs:domain aas:AdminShell ;
                   rdfs:range aas:Dimension ;
                   rdfs:comment "Connects the Admin Shell with the different RAMI4.0 Dimensions"@en ;
                   rdfs:label "is Connected To"@en .


###  https://admin-shell.io/aas/2/0/rdf#mimeType
aas:mimeType rdf:type owl:ObjectProperty ;
              rdfs:comment """Mime type of the content of the BLOB.
The mime type states which file extension the file has.
Valid values are e.g. “application/json”, “application/xls”, ”image/jpg”
The allowed values are defined as in RFC2046.

or

Mime type of the content of the File."""@en ;
              rdfs:label "mimeType"^^xsd:string ;
              rdfs:seeAlso "http://uri4uri.net/vocab.html/#MimetypeDatatype"^^xsd:string .


###  https://admin-shell.io/aas/2/0/rdf#object
aas:object rdf:type owl:ObjectProperty ;
            rdfs:comment "Element to which permission shall be assigned."@en ;
            rdfs:label "has object"^^xsd:string .


###  https://admin-shell.io/aas/2/0/rdf#objectAttribute
aas:objectAttribute rdf:type owl:ObjectProperty ;
                     rdfs:comment "A data element that further classifies an object."@en ;
                     rdfs:label "objectAttribute"^^xsd:string .


###  https://admin-shell.io/aas/2/0/rdf#out
aas:out rdf:type owl:ObjectProperty ;
         rdfs:comment "out is the output paramter of the Operation"@en ;
         rdfs:label "out"@en .


###  https://admin-shell.io/aas/2/0/rdf#parent
aas:parent rdf:type owl:ObjectProperty ;
            rdfs:comment """Reference to the next referable parent element of the element. Constraint AASd-004: Add parent in case of non-identifiable elements.
Note: This element is used to ease navigation in the model and thus it enables more performant"""@en ;
            rdfs:label "parent"@en .


###  https://admin-shell.io/aas/2/0/rdf#preferredName
aas:preferredName rdf:type owl:ObjectProperty ;
                   rdfs:comment "This is the preferredName of a ConceptDescription object"@en ;
                   rdfs:label "preferredName"^^xsd:string .


###  https://admin-shell.io/aas/2/0/rdf#qualifierType
aas:qualifierType rdf:type owl:ObjectProperty .


###  https://admin-shell.io/aas/2/0/rdf#qualifierValue
aas:qualifierValue rdf:type owl:ObjectProperty ;
                    rdfs:comment """The qualifier value is the value of the qualifier.
Constraint AASd-006: if both, the value and the valueId are present then the value needs to be identical to the short name of the referenced coded value in qualifierValueId."""@en .


###  https://admin-shell.io/aas/2/0/rdf#second
aas:second rdf:type owl:ObjectProperty ;
            rdfs:comment "Second element in the relationship taking the role of the object."@en ;
            rdfs:label "second"^^xsd:string .


###  https://admin-shell.io/aas/2/0/rdf#selectableEnvironmentAttributes
aas:selectableEnvironmentAttributes rdf:type owl:ObjectProperty ;
                                     rdfs:comment """Reference to a submodel defining which environment attributes can be accessed via the permission rules defined for the AAS, i.e. attributes that are not describing the asset itself.
Default: reference to the submodel referenced via
defaultEnvironmentAttributes"""@en ;
                                     rdfs:label "selectableEnvironmentAttributes"^^xsd:string .


###  https://admin-shell.io/aas/2/0/rdf#submodelElement
aas:submodelElement rdf:type owl:ObjectProperty ;
                     rdfs:range aas:SubmodelElement ;
                     rdfs:comment """A submodel consists of zero or more
submodel elements."""@en ;
                     rdfs:label "has Submodel Element"@en .


###  https://admin-shell.io/aas/2/0/rdf#targetObjectAttributes
aas:targetObjectAttributes rdf:type owl:ObjectProperty ;
                            rdfs:comment "Target object attributes that need to be fulfilled so that the access permissions apply to the accessing subject."@en ;
                            rdfs:label "targetObjectAttributes"^^xsd:string .


###  https://admin-shell.io/aas/2/0/rdf#targetSubjectAttributes
aas:targetSubjectAttributes rdf:type owl:ObjectProperty ;
                             rdfs:comment "Target subject attributes that need to be fulfilled by the accessing subject to get the permissions defined by this rule."@en ;
                             rdfs:label "targetSubjetAtrtibutes"^^xsd:string .


###  https://admin-shell.io/aas/2/0/rdf#trustAnchor
aas:trustAnchor rdf:type owl:ObjectProperty ;
                 rdfs:comment "Trust anchor of AAS, typically certificates."@en ;
                 rdfs:label "trustAnchor"^^xsd:string .


###  https://admin-shell.io/aas/2/0/rdf#value
aas:value rdf:type owl:ObjectProperty ;
           rdfs:comment "The key value, for example an IRDI if the idType=IRDI."@en ;
           rdfs:label "keyValue"^^xsd:string .


#################################################################
#    Data properties
#################################################################

###  http://purl.org/dc/terms/hasVersion
dcterms:hasVersion rdf:type owl:DatatypeProperty .


###  http://purl.org/dc/terms/identifier
dcterms:identifier rdf:type owl:DatatypeProperty .


###  http://www.wurvoc.org/vocabularies/om-1.8/hasNumericalValue
om:hasNumericalValue rdf:type owl:DatatypeProperty .


###  https://admin-shell.io/aas/2/0/rdf#allowDuplicates
aas:allowDuplicates rdf:type owl:DatatypeProperty ;
                     rdfs:comment """If allowDuplicates=true then it is allowed that the collection contains the same element several times.
Default = false"""@en ;
                     skos:altLabel "allow duplicates"^^xsd:string .


###  https://admin-shell.io/aas/2/0/rdf#assetId
aas:assetId rdf:type owl:DatatypeProperty ;
             rdfs:subPropertyOf dcterms:identifier .


###  https://admin-shell.io/aas/2/0/rdf#creationDate
aas:creationDate rdf:type owl:DatatypeProperty ;
                  rdfs:domain aas:Submodel ;
                  rdfs:range xsd:dateTime ;
                  skos:definition "Date when an Agent(Person or Software) creates to the Entity/Object related data. It correspond to the Creator concept of OMM"@en ;
                  skos:prefLabel "has Creator"@en .


###  https://admin-shell.io/aas/2/0/rdf#definition
aas:definition rdf:type owl:DatatypeProperty ;
                rdfs:label "This is the definition that is contained in the conceptDescription."@en ,
                           "has definition"^^xsd:string .


###  https://admin-shell.io/aas/2/0/rdf#description
aas:description rdf:type owl:DatatypeProperty .


###  https://admin-shell.io/aas/2/0/rdf#hasLocal
aas:hasLocal rdf:type owl:DatatypeProperty ;
              rdfs:comment "Denotes if the key references a model element of the same AAS (=true) or not (=false). In case of local = false the key may reference a model element of another AAS or an entity outside any AAS that has a global unique id."@en ;
              rdfs:label "has local"^^xsd:string .


###  https://admin-shell.io/aas/2/0/rdf#id
aas:id rdf:type owl:DatatypeProperty ;
        rdfs:subPropertyOf dcterms:identifier ;
        rdfs:comment "A globally unique identifier which is NOT a URI."@en ;
        rdfs:label "identification"@en .


###  https://admin-shell.io/aas/2/0/rdf#idShort
aas:idShort rdf:type owl:DatatypeProperty ;
             rdfs:subPropertyOf dcterms:identifier .


###  https://admin-shell.io/aas/2/0/rdf#isCaseOf
aas:isCaseOf rdf:type owl:DatatypeProperty ;
              rdfs:subPropertyOf dcterms:identifier .


###  https://admin-shell.io/aas/2/0/rdf#isDescribedWith
aas:isDescribedWith rdf:type owl:DatatypeProperty ;
                     rdfs:seeAlso aas:asset ;
                     owl:deprecated "true"^^xsd:boolean ;
                     skos:definition "Points to the Standard used to describe a given object"@en ;
                     skos:prefLabel "Is Described With"@en .


###  https://admin-shell.io/aas/2/0/rdf#logs
aas:logs rdf:type owl:DatatypeProperty ;
          rdfs:range xsd:string ;
          skos:prefLabel "logs"@en .


###  https://admin-shell.io/aas/2/0/rdf#ordered
aas:ordered rdf:type owl:DatatypeProperty ;
             rdfs:comment """If ordered=false then the elements in the property collection are not ordered. If ordered=true then the elements in the collection are ordered.
Default = false"""@en ;
             rdfs:label "ordered"^^xsd:string .


###  https://admin-shell.io/aas/2/0/rdf#publishedURL
aas:publishedURL rdf:type owl:DatatypeProperty .


###  https://admin-shell.io/aas/2/0/rdf#revision
aas:revision rdf:type owl:DatatypeProperty ;
              rdfs:subPropertyOf dcterms:hasVersion ;
              rdfs:comment "Revision of the element. Constraint AASd-005: A revision requires a version. This means, if there is no version there is no revision neither."@en ;
              rdfs:label "revision"@en .


###  https://admin-shell.io/aas/2/0/rdf#semanticId
aas:semanticId rdf:type owl:DatatypeProperty ;
                rdfs:subPropertyOf dcterms:identifier .


###  https://admin-shell.io/aas/2/0/rdf#version
aas:version rdf:type owl:DatatypeProperty ;
             rdfs:subPropertyOf dcterms:hasVersion ;
             rdfs:comment "Version of the element."@en ;
             rdfs:label "version"@en .


#################################################################
#    Classes
#################################################################

###  https://admin-shell.io/aas/2/0/rdf#AccessControlPolicyPoints
aas:AccessControlPolicyPoints rdf:type owl:Class ;
                               rdfs:comment "Container for access control policy points."@en ;
                               rdfs:label "Access ControlPolicy Points"^^xsd:string .


###  https://admin-shell.io/aas/2/0/rdf#AdminShell
aas:AdminShell rdf:type owl:Class ;
                rdfs:subClassOf aas:HasDataSpecification ,
                                aas:Identifiable ;
                dce:source "This definition comprises material from RAMI4.0."@en ;
                rdfs:label "Admin Shell"@en ;
                skos:altLabel "Administration Shell"@en ,
                              "Asset Administration Shell"@en ;
                skos:definition "Describes the Administration Shell for Assets, Products, Components, e.g. Machines"@en ;
                skos:prefLabel "Verwaltungsschale"^^xsd:string .


###  https://admin-shell.io/aas/2/0/rdf#AdministrativeInformation
aas:AdministrativeInformation rdf:type owl:Class ;
                               rdfs:subClassOf aas:DataSpecification ;
                               rdfs:comment """Every Identifiable may have administrative information. Administrative information includes for example
 Information about the version of the element
 Information about who created or who made the last change to the element
 Information about the languages available in case the element contains text, for translating purposed also themmaster or default language may be defined
In the first version of the AAS metamodel only version information as defined by IEC 61360 is defined. In later versions additional attributes may be added."""@en ;
                               rdfs:label "Administrative Information"^^xsd:string .


###  https://admin-shell.io/aas/2/0/rdf#Asset
aas:Asset rdf:type owl:Class ;
           rdfs:subClassOf aas:HasDataSpecification ,
                           aas:HasKind ,
                           aas:Identifiable .


###  https://admin-shell.io/aas/2/0/rdf#AssetKind
aas:AssetKind rdf:type owl:Class ;
               rdfs:subClassOf aas:Dimension ;
               rdfs:comment """The RAMI4.0 model features one, generalized life-cycle axis, which was derived from IEC 62890. The basic idea is to distinguish for all assets within Industrie 4.0 between possible types and instance. This makes it possible to apply the type/instance distinction for all elements such as material type/material instance, product type/product instance, machine type/ machine instance and more. Business related information will be handled on the 'Business' layer of the
RAMI4.0 model, as well, covering also order details and workflows, again with types/ instances."""@en ;
               rdfs:label "Asset Kind"@en .


###  https://admin-shell.io/aas/2/0/rdf#Blob
aas:Blob rdf:type owl:Class ;
          rdfs:subClassOf aas:DataElement ;
          rdfs:comment "A BLOB is a data element that represents a file that is contained with its source code in the value attribute."@en ;
          rdfs:label "BlobDataElement"@en .


###  https://admin-shell.io/aas/2/0/rdf#ConceptDescription
aas:ConceptDescription rdf:type owl:Class ;
                        rdfs:subClassOf aas:HasDataSpecification ,
                                        aas:Identifiable ;
                        dce:description "\"The AAS itself can also define its own dictionary that contains semantic definitions of its submodel elements. These semantic definitions are called concept descriptions (ConceptDescription). It is optional whether an AAS defines its own concept dictionary (ConceptDictionary) or not.\""@en .


###  https://admin-shell.io/aas/2/0/rdf#ConceptDictionary
aas:ConceptDictionary rdf:type owl:Class ;
                       rdfs:subClassOf aas:Referable ;
                       rdfs:comment "A dictionary contains elements that can be reused. The concept dictionary contains concept descriptions. Typically a concept description dictionary of an AAS contains only concept descriptions of elements used within submodels of the AAS."@en ;
                       rdfs:label "Concept Dictionary" .


###  https://admin-shell.io/aas/2/0/rdf#DataElement
aas:DataElement rdf:type owl:Class ;
                 rdfs:subClassOf aas:SubmodelElement ;
                 rdfs:comment "A data element is a submodel element that is not further composed out of other submodel elements. A data element is a submodel element that has a value. The type of value differs for different subtypes of data elements."@en ;
                 rdfs:label "DataElement"^^xsd:string ;
                 skos:note "abstract" .


###  https://admin-shell.io/aas/2/0/rdf#DataSpecification
aas:DataSpecification rdf:type owl:Class ;
                       rdfs:comment "Element that can have data specification templates. A template defines the additional attributes an element may or shall have."@en ;
                       rdfs:label "DataSpecification"@en ;
                       skos:note "abstract"@en .


###  https://admin-shell.io/aas/2/0/rdf#Dimension
aas:Dimension rdf:type owl:Class .


###  https://admin-shell.io/aas/2/0/rdf#File
aas:File rdf:type owl:Class ;
          rdfs:subClassOf aas:DataElement ;
          rdfs:comment "A File is a data element that represents a file via its path description."@en ;
          rdfs:label "FileDataElement"@en .


###  https://admin-shell.io/aas/2/0/rdf#Formula
aas:Formula rdf:type owl:Class ;
             dce:description "A formula is used to describe constraints by a logical expression."@en ;
             rdfs:label "Formula"@en .


###  https://admin-shell.io/aas/2/0/rdf#HasDataSpecification
aas:HasDataSpecification rdf:type owl:Class ;
                          rdfs:comment "Element that can have data specification templates. A template defines the additional attributes an element may or shall have."@en ;
                          rdfs:label "Has Data Specification"@en ;
                          skos:prefLabel "Data Specification"@en .


###  https://admin-shell.io/aas/2/0/rdf#HasKind
aas:HasKind rdf:type owl:Class ;
             rdfs:comment "An element with a kind is an element that can either represent a type or an instance. Default for an element is that it is representing an instance."@en ;
             rdfs:label "Has Kind"@en .


###  https://admin-shell.io/aas/2/0/rdf#Identifiable
aas:Identifiable rdf:type owl:Class ;
                  rdfs:subClassOf aas:Referable ;
                  rdfs:comment "An element that has a globally unique identifier."@en ;
                  rdfs:label "Identifiable"@en ;
                  skos:note "abstract"@en .


###  https://admin-shell.io/aas/2/0/rdf#Key
aas:Key rdf:type owl:Class ;
         rdfs:comment "A key is a reference to an element by its id."@en ;
         rdfs:label "Key"^^xsd:string .


###  https://admin-shell.io/aas/2/0/rdf#ObjectAttributes
aas:ObjectAttributes rdf:type owl:Class ;
                      rdfs:comment "A set of data elements that describe object attributes. These attributes need to refer to a data element within an existing submodel."@en ;
                      rdfs:label "Object Attributes"^^xsd:string .


###  https://admin-shell.io/aas/2/0/rdf#Operation
aas:Operation rdf:type owl:Class ;
               rdfs:subClassOf aas:SubmodelElement ;
               rdfs:comment "An operation is a submodel element with input and output variables."@en ;
               rdfs:label "Operation"@en .


###  https://admin-shell.io/aas/2/0/rdf#OperationVariable
aas:OperationVariable rdf:type owl:Class ;
                       rdfs:subClassOf aas:SubmodelElement ;
                       dce:description "An operation variable is a submodel element that is used as input or output variable of an operation."@en ;
                       rdfs:label "Operation Variable"^^xsd:string .


###  https://admin-shell.io/aas/2/0/rdf#Order
aas:Order rdf:type owl:Class ;
           skos:definition "Each order for manufacturing runs through a life cycle and its specifics necessarily have an impact on the production facility during performance of the order"@en ;
           skos:note "TODO: Delete?" ;
           skos:prefLabel "Order"@en .


###  https://admin-shell.io/aas/2/0/rdf#Property
aas:Property rdf:type owl:Class ;
              rdfs:comment "A property is a data element that has a single value."@en ;
              rdfs:label "Property"@en ;
              skos:note "TODO: delete?" .


###  https://admin-shell.io/aas/2/0/rdf#PropertyValueType
aas:PropertyValueType rdf:type owl:Class ;
                       dce:description """The qualifier value is the value of the qualifier.
Constraint AASd-006: if both, the value and the valueId are present then the value needs to be identical to the short name of the referenced coded value in qualifierValueId."""@en .


###  https://admin-shell.io/aas/2/0/rdf#Qualifier
aas:Qualifier rdf:type owl:Class ;
               dce:description "A qualifier is a type-value pair that makes additional statements w.r.t. the value of the element."@en ;
               rdfs:label "Qualifier"@en .


###  https://admin-shell.io/aas/2/0/rdf#Referable
aas:Referable rdf:type owl:Class ;
               rdfs:comment "An element that is referable by its idShort. This id is not globally unique. This id is unique within the name space of the element."@en ;
               rdfs:label "Referable"@en ;
               skos:note "abstract" .


###  https://admin-shell.io/aas/2/0/rdf#Reference
aas:Reference rdf:type owl:Class ;
               rdfs:comment """Reference to either a model element of the same or another AAs or to an external entity.
A reference is an ordered list of keys, each key referencing an element. The complete list of keys may for example be concatenated to a path that then gives unique access to an element or entity."""@en ;
               rdfs:label "Reference"^^xsd:string .


###  https://admin-shell.io/aas/2/0/rdf#ReferenceElement
aas:ReferenceElement rdf:type owl:Class ;
                      dce:description "A reference element is a data element that defines a reference to another element within the same or another AAS or a reference to an external object or entity."@en ;
                      rdfs:label "Reference Element"^^xsd:string .


###  https://admin-shell.io/aas/2/0/rdf#RelationshipElement
aas:RelationshipElement rdf:type owl:Class ;
                         rdfs:subClassOf aas:SubmodelElement ;
                         dce:description "A relationship element is used to define a relationship between two referable elements."@en ;
                         rdfs:label "RelationshipElement"@en .


###  https://admin-shell.io/aas/2/0/rdf#Security
aas:Security rdf:type owl:Class ;
              rdfs:comment "Container for security relevant information of the AAS."@en ;
              rdfs:label "Security"^^xsd:string .


###  https://admin-shell.io/aas/2/0/rdf#Submodel
aas:Submodel rdf:type owl:Class ;
              rdfs:subClassOf aas:HasDataSpecification ,
                              aas:HasKind ,
                              aas:Identifiable ;
              rdfs:comment """A Submodel defines a specific aspect of the asset represented by the AAS.
A submodel is used to structure the virtual representation and technical functionality of an Administration Shell into distinguishable parts. Each submodel refers to a well-defined domain or subject matter.
Submodels can become standardized and thus become submodels types. Submodels can have different life-cycles."""@en ,
                           "Describe the different types of Data related to the I4.0 Asset"@en ;
              rdfs:label "Submodel"@en .


###  https://admin-shell.io/aas/2/0/rdf#SubmodelElement
aas:SubmodelElement rdf:type owl:Class ;
                     rdfs:subClassOf aas:HasDataSpecification ,
                                     aas:HasKind ,
                                     aas:Identifiable ;
                     rdfs:comment "A submodel element is an element suitable for the description and differentiation of assets."@en ;
                     rdfs:label "Submodel Element"^^xsd:string ;
                     skos:note "abstract"@en .


###  https://admin-shell.io/aas/2/0/rdf#SubmodelElementCollection
aas:SubmodelElementCollection rdf:type owl:Class ;
                               rdfs:subClassOf aas:SubmodelElement ;
                               rdfs:comment "A submodel element collection is a set or list of submodel elements."@en ;
                               rdfs:label "SubmodelElementCollection"@en .


###  https://admin-shell.io/aas/2/0/rdf#Value
aas:Value rdf:type owl:Class ;
           rdfs:comment """Current value that can be specified through an instanced submodel (for 
instance in station 2) or through the asset, for example."""@en ;
           rdfs:label "Value"@en ;
           skos:note "maybe 'containedElement'?"@en .


###  https://admin-shell.io/aas/2/0/rdf#View
aas:View rdf:type owl:Class ;
          rdfs:subClassOf aas:HasDataSpecification ,
                          aas:Referable ;
          rdfs:comment "Different views associated to the Administration Shell via the Submodels"@en ;
          rdfs:isDefinedBy "https://www.plattform-i40.de/I40/Redaktion/DE/Downloads/Publikation/hm-2018-trilaterale-coop.html"@de ;
          rdfs:label "Sicht"@de ,
                     "View"@en .


#################################################################
#    Individuals
#################################################################

###  https://admin-shell.io/aas/2/0/rdf#Asset
aas:Asset rdf:type owl:NamedIndividual .


###  https://admin-shell.io/aas/2/0/rdf#Instance
aas:Instance rdf:type owl:NamedIndividual .


###  https://admin-shell.io/aas/2/0/rdf#Type
aas:Type rdf:type owl:NamedIndividual ,
                   aas:AssetKind ;
          rdfs:comment """The RAMI4.0 model features one, generalized life-cycle axis, which was derived from IEC 62890. The basic idea is to distinguish for all assets within Industrie 4.0 between possible types and instance. This makes it possible to apply the
type/instance distinction for all elements such as material type/material instance, product type/product instance, machine type/ machine instance and more. Business related information will be handled on the 'Business' layer of the
RAMI4.0 model, as well, covering also order details and workflows, again with types/ instances."""@en ;
          rdfs:label "Type"@en ;
          skos:altLabel "Asset Type"^^xsd:string .


#################################################################
#    Annotations
#################################################################

om:hasNumericalValue rdfs:label "has numerical value"@en .


aas:Asset skos:altLabel "Object"@en ;
           skos:definition "Clearly identifiable asset for the Administration Shell"@en ;
           skos:altLabel "Entity"@en ;
           skos:prefLabel "Asset"@en ;
           skos:definition "Eindeutig identifizierbarer Gegenstand, der aufgrund seiner Bedeutung in der Informationswelt verwaltet wird"@de ;
           rdfs:comment """An Asset describes meta data of an asset that is represented by an AAS.
The asset may either represent an asset type or an asset instance.
The asset has a globally unique identifier plus – if needed – additional domain specific (proprietary) identifiers."""@en ;
           skos:note "Objects may be known in the form of a type or of an instance. An object in the planning phase is known as a type"@en ;
           skos:altLabel "Entität"@de .


aas:assetId owl:deprecated "true"^^xsd:boolean ;
             rdfs:label "id"@en ;
             rdfs:comment "The unique identifier of an asset. Note the difference between the 'asset ID' idenitfier and the URIs for the resources."@en .


aas:description rdfs:comment "Description or comments on the element. The description can be provided in several languages."@en ;
                 skos:prefLabel "has Description"@en .


aas:idShort rdfs:label "idShort"@en ;
             owl:deprecated "true"^^xsd:boolean .


aas:semanticId rdfs:comment "The semantic id might refer to an external information source, which explains the formulation of the submodel (for example an PDF if a standard)"@en ;
                rdfs:label "semanticId"@en ;
                rdfs:comment "Points to the Expression Semantic of the Submodels"@en ;
                skos:altLabel "has Semantic Expression"@en ;
                skos:prefLabel "has semantic ID"@en .


###  Generated by the OWL API (version 4.2.8.20170104-2310) https://github.com/owlcs/owlapi
